fixed definitions

.coqdeps.d
@@ -1,7 +1,7 @@
 NonEmpty.vo NonEmpty.glob NonEmpty.v.beautified: NonEmpty.v
 NonEmpty.vio: NonEmpty.v
-CGS.vo CGS.glob CGS.v.beautified: CGS.v NonEmpty.vo
-CGS.vio: CGS.v NonEmpty.vio
+CGS.vo CGS.glob CGS.v.beautified: CGS.v
+CGS.vio: CGS.v
 ATL.vo ATL.glob ATL.v.beautified: ATL.v CGS.vo
 ATL.vio: ATL.v CGS.vio
 VNM.vo VNM.glob VNM.v.beautified: VNM.v ATL.vo
