CGS.v
@@ -2,9 +2,8 @@ Require Export List.
 Require Export Classical.
 Require Export Decidable.
 Require Export FunctionalExtensionality.
+Require Export Streams.
 
-
-Require Export NonEmpty.
 Require Import Coq.Lists.List Coq.Bool.Bool.
 
 Import Coq.Lists.List.ListNotations.
@@ -14,11 +13,22 @@ Scheme Equality for list.
 Parameter State : Set.
 Parameter Player : Set.
 Parameter Observable : Set.     (* set of atomic truths that can hold at a given state. *)
-Parameter Move : Set.           (* alphabet of moves individual players can make. 
-*)
+Parameter Move : Set.           (* alphabet of moves individual players can make.*)
+
+
+
 Parameter beq_state : State -> State -> bool.
 Parameter beq_player : Player -> Player -> bool.
 Parameter beq_observable : Observable -> Observable -> bool.
+
+Axiom beq_state_refl : forall (q:State), beq_state q q = true.
+Axiom beq_player_refl : forall (p:Player), beq_player p p = true.
+Axiom beq_observable_refl : forall (o:Observable), beq_observable o o = true.
+
+Axiom beq_state_Prop : forall (q1 q2:State), beq_state q1 q2 = true -> q1 = q2.
+Axiom beq_player_Prop : forall (p1 p2:Player), beq_player p1 p2 = true -> p1 = p2.
+Axiom beq_obervable_Prop : forall (o1 o2:Observable), beq_observable o1 o2 = true -> o1 = o2.
+
 (* type corresponding to the set of moves each player makes. *)
 Definition move_vec := State -> Player -> Move.
 
@@ -51,144 +61,37 @@ Definition succ (g:CGS) (q q':State) :=
 
 (* Computations are nonempty sequences of states [l] where every [l_(i+1)] is a successor of [l_i]. *)
 
+Fixpoint Stream_firstn {A:Type} (i:nat) (s:Stream A) : list A :=
+  match i with
+  | 0 => nil
+  | S i => match s with
+           | Cons a b => a :: Stream_firstn i b
+           end
+  end.
+  
 
 (* [computation_property_fix] checks that successive states are successors according to the above property. *)
 
-Inductive computation_property: CGS -> State -> nonempty State -> Prop :=
-| computation_property_one: forall (g: CGS) (s: State),
-    computation_property g s (s:::nil)
-| computation_property_cons: forall (g: CGS) (ss: list State) (s1 s2: State)
-    (FIXSUCC: computation_property g s2 (s2 :::ss ))
+Inductive computation_property_finite: CGS -> State -> list State -> Prop :=
+| computation_property_finite_one : forall (g:CGS) (s : State),
+    computation_property_finite g s (s::nil)
+| computation_property_finite_cons: forall (g: CGS) (ss: list State) (s1 s2: State)
+    (FIXSUCC: computation_property_finite g s2 (s2::ss))
     (SUCC: succ g s1 s2),
-    computation_property g s1 (s1:::s2::ss).
+    computation_property_finite g s1 (s1::s2::ss).
+
+CoInductive computation_property: CGS -> State -> Stream State -> Prop :=
+| computation_property_cons: forall (g: CGS) (ss: Stream State) (s1 s2: State)
+    (FIXSUCC: computation_property g s2 (Cons s2 ss))
+    (SUCC: succ g s1 s2),
+    computation_property g s1 (Cons s1 (Cons s2 ss)).
 
 
+Theorem computation_property_prefix : forall (g:CGS) (q:State) (l:Stream State) (i:nat),
+    computation_property g q l -> computation_property_finite g q (Stream_firstn (S i) l).
+Proof.
+  Admitted.
 
-(* Subset type of [list State] where [computation_property] holds. *)
-(* )Definition computation (g:CGS) (q:State) : Set := {l:list State | computation_property g q l}.
- *)
-
-
-(* If a [list State] is a [q]-computation, that same [list State] cons'ed with State [a] is an [a]-computation. *)
-(* Theorem computation_property_cons : *)
-(*   forall (g:CGS) (l:list State) (q a b:State), *)
-(*     computation_property g q (b::l) /\ succ g a b -> computation_property g a (a::b::l). *)
-(* Proof. *)
-(*   intros. destruct H. destruct H. unfold computation_property. split. *)
-(*   - reflexivity. *)
-(*   - simpl. split. *)
-(*     + apply H0. *)
-(*     + simpl in H1. apply H1. *)
-(* Qed. *)
-
-(* (* A list has length > 0 iff there exists a head to the list.*) *)
-(* Theorem  length_hd_error : forall (A:Type) (l:list A), 1 <= length l <-> exists y:A, hd_error l = Some y. *)
-(* Proof. *)
-(* intros. split. *)
-(* - induction l. *)
-(*   + intros. inversion H. *)
-(*   + intros. exists a. reflexivity. *)
-(* - intros. destruct H. assert (x::(tl l) = l). *)
-(*   { symmetry. apply hd_error_tl_repr. split. *)
-(*     - apply H. *)
-(*     - reflexivity. *)
-(*   } *)
-(*   rewrite <- H0. simpl. induction (length (tl l)). *)
-(*   + reflexivity. *)
-(*   + apply le_S. apply IHn. *)
-(* Qed. *)
-
-(* (* The head of a list [b0++b1] is the head of list [b0] if [b0] is nonempty.*) *)
-(* Theorem hd_error_app : forall (b0 b1: list State) (a:State), hd_error b0 = Some a -> (hd_error (b0 ++ b1)) = Some a. *)
-(*   { *)
-(*     intros. induction b0. *)
-(*     - inversion H. *)
-(*     - simpl. simpl in H. apply H. *)
-(*   } *)
-(* Qed. *)
-
-(* (* If [computation_property] holds for [l0++l1] and [l0] is nonempty, [computation_property] holds for [l0]. *) *)
-(* Theorem computation_property_app : *)
-(*   forall (g:CGS) (q:State) (l0 l1: list State), *)
-(*     (1 <= (length l0)) -> computation_property g q (l0 ++ l1) -> computation_property g q l0. *)
-(* Proof. *)
-(*   intros. destruct H0. unfold computation_property. generalize dependent q. induction l0. *)
-(*   - intros. inversion H. *)
-(*   - intros. split. *)
-(*     + simpl in H0. simpl. apply H0. *)
-(*     + simpl. simpl in H1. simpl in H0. inversion H. *)
-(*       * *)
-(*         assert (hd_error l0 = None). *)
-(*         { *)
-(*           symmetry in H3. apply length_zero_iff_nil in H3. *)
-(*           rewrite H3. reflexivity. *)
-(*         } *)
-(*         rewrite H2. apply I. *)
-(*       *  *)
-(*         assert (length l0 > 0). *)
-(*         { unfold gt. unfold lt. apply H3. } *)
-(*         apply length_hd_error in H3. destruct H3. apply (hd_error_app l0 l1 x) in H3. *)
-(*         rewrite H3 in H1. destruct H1. apply (IHl0 H4 H5 x) in H3. *)
-(*         destruct H3. *)
-(*         rewrite H3. split. *)
-(*         -- apply H1. *)
-(*         -- apply H6. *)
-(* Qed. *)
-
-(* (* The nonempty prefix of a [q]-computation is a [q]-computation. *) *)
-(* Theorem computation_property_prefix : *)
-(*   forall (g:CGS) (n:nat) (q:State) (l:computation g q), *)
-(*     computation_property g q (firstn (S n) (proj1_sig l)). *)
-(* Proof. *)
-(*   intros. destruct l. unfold proj1_sig. destruct c. *)
-(*   pose proof (hd_error_app (firstn (S n) x) (skipn (S n) x) q) as H1. *)
-(*   assert ((hd_error (firstn (S n) x)) = Some q). *)
-(*   { *)
-(*     simpl. destruct x. *)
-(*     - apply H. *)
-(*     - simpl. simpl in H. apply H. *)
-(*   } *)
-(*   apply H1 in H2. *)
-(*   destruct (length_hd_error State x). *)
-(*   assert (exists y, hd_error x = Some y). *)
-(*   { exists q. apply H. } *)
-(*   apply H4 in H5. *)
-(*   pose proof (@computation_property_app g q (firstn (S n) x) (skipn (S n) x)). *)
-(*   assert (1 <= length (firstn (S n) x)). *)
-(*   { *)
-(*     induction x. *)
-(*     - inversion H. *)
-(*     - simpl. induction (firstn n x). *)
-(*       + reflexivity. *)
-(*       + simpl. apply le_S. apply IHl. *)
-(*   } *)
-(*   assert (@computation_property g q x). *)
-(*   { *)
-(*     unfold computation_property. split. *)
-(*     - apply H. *)
-(*     - apply H0. *)
-(*   } *)
-(*   rewrite firstn_skipn in H6. *)
-(*   apply (H6 H7 H8). *)
-(* Qed. *)
-
-(* (* A function generating the [n+1]-long prefix of a [q]-computation.*) *)
-(* Definition computation_prefix *)
-(*            (g:CGS) *)
-(*            (q:State) *)
-(*            (l: computation g q) *)
-(*            (n:nat) *)
-(*            : computation g q *)
-(* := *)
-(*   @exist (list State) *)
-(*          (computation_property g q)(* (fun l => computation_property g q l) *) *)
-(*          (firstn (S n) (proj1_sig l)) *)
-(*          (computation_property_prefix g n q l). *)
-
-(* Check computation_prefix. *)
-
-
-(* There is always a move available called [nothing], which if performed by every player fails to change state. *)
 
 (* A coalition is a set of players. *)
 Definition coalition : Set := Player -> bool.
@@ -208,7 +111,13 @@ Parameter nothing: Move.
 Axiom nothing_always_enabled : forall (g:CGS) (q:State) (p:Player), g.(e) q p nothing = true.
 Axiom nothing_does_nothing : forall (g:CGS) (q:State), g.(d) q (fun _ _ => nothing) = q.
 
+CoFixpoint sq (q:State) : Stream State :=
+  Cons q (sq q).
 
+Theorem computation_property_sq : forall g q, computation_property g q (sq q).
+Proof.
+Admitted.
+  
 (* A strategy is a function from computations to moves, representing what a player would do in a particular play-through. *)
 
 (* Inductive strategy (g:CGS) (p:Player) : (nonempty State) -> Move -> Set := *)
@@ -220,11 +129,11 @@ Axiom nothing_does_nothing : forall (g:CGS) (q:State), g.(d) q (fun _ _ => nothi
 (*   fun l => strat g p l nothing (nothing_always_enabled g (nonempty_last l) p). *)
 
 
-Definition strategy (g:CGS) (p:Player) : Set := forall (l:nonempty State) (q:State) (CPL: computation_property g q l), Move.
+Definition strategy (g:CGS) (p:Player) : Set := forall (l:list State) (q:State) (CPL: computation_property_finite g q l), Move.
 
 Definition strategy_legal (g:CGS) (p:Player) (s:strategy g p) :=
-  forall (l:nonempty State) (q:State) (CPL: computation_property g q l),
-    g.(e) (nonempty_last l) p (s l q CPL) = true.
+  forall (l:list State) (q:State) (CPL: computation_property_finite g q l),
+    g.(e) (last l q) p (s l q CPL) = true.
 
 Definition strat_nothing (g: CGS) (p:Player) : strategy g p :=
   fun l _ _ => nothing.
@@ -238,61 +147,41 @@ Proof.
 Qed.
 
 (* [strategy_set] is a type representing unique strategies only of members in the coalition. *)
-Inductive strategy_set (g:CGS) (c:coalition) : Set :=
-| strat_set : forall (p:Player)
-                     (COAL: c p = true)
-                     (s: strategy g p)
-                     (SL: strategy_legal g p s),
-    strategy_set g c.
+Definition strategy_set (g:CGS) (c:coalition) :=
+  forall (p:Player)
+         (COAL: c p = true),
+    {s: strategy g p | strategy_legal g p s}.
 
 
 (* Strategy set where members of the coalition do nothing. *)
-Definition ss_nothing (g:CGS) (c:coalition) := fun p COAL => strat_set g c p COAL (strat_nothing g p) (nothing_always_legal g p).
+Definition ss_nothing (g:CGS) (c:coalition) : strategy_set g c := fun p COAL => exist (strategy_legal g p) (strat_nothing g p) (nothing_always_legal g p).
 
 Check ss_nothing.
+
 
 (* Whether a particular move vector obeys a given strategy set. *)
 Definition strategy_set_enabled
            (g:CGS)
            (c:coalition)
            (ss:strategy_set g c)
-           (l:nonempty State)
+           (l:list State)
            (q:State)
-           (CPL: computation_property g q l)
-           (mv:move_vec) :=
-  match ss with
-  | strat_set _ _ p _ s _ =>  mv (nonempty_last l) p  = s l q CPL
+           (CPL: computation_property_finite g q l)
+           (m:move_vec) :=
+  forall (p:Player) (COAL: c p = true),
+  match (ss p COAL) with
+  | exist _ s _ =>  m (last l q) p  = s l q CPL
   end.
 (* TODO make [strategy_set], [strategy] inductive *)
 
 
-Inductive outcomes (g:CGS) (c: coalition) : (strategy_set g c) -> nonempty State -> Prop :=
-| outcomes_two : forall (ss:strategy_set g c) (q1 q2:State)
-                        (m: move_vec)
-                        (CPL: computation_property g q1 (q1:::q2::nil))
-                        (ENABLED: strategy_set_enabled g c ss (q1:::q2::nil) q1 CPL m)
-                        (DELTA: g.(d) q1 m = q2),
-    outcomes g c ss (q1:::q2::nil)
-| outcomes_cons : forall (ss:strategy_set g c) (q:State)
-                         (l:nonempty State)
+CoInductive outcomes (g:CGS) (c: coalition) : (strategy_set g c) -> Stream State -> Prop :=
+| outcomes_cons : forall (ss:strategy_set g c) (q1 q2:State)
+                         (l:Stream State)
                          (m:move_vec)
-                         (CPL: computation_property g q (nonempty_cons q l))
-                         (ENABLED : strategy_set_enabled g c ss (nonempty_cons q l) q CPL m)
-                         (OUT: outcomes g c ss l),
-      outcomes g c ss (nonempty_cons q l).
+                         (CPL: computation_property g q1 (Cons q1 (Cons q2 l)))
+                         (ENABLED : strategy_set_enabled g c ss (q1::nil) q1 (computation_property_prefix g q1 (Cons q1 (Cons q2 l)) 0 CPL) m)
+                         (DELTA: g.(d) q1 m = q2)
+                         (OUT: outcomes g c ss (Cons q2 l)),
+      outcomes g c ss (Cons q1 (Cons q2 l)).
            
-                        (* TODO finish redefining outcomes *)
-
-(* Property checking whether a given computation obeys a strategy set in all successive states. *)
-(* Definition outcomes (g:CGS) (q:State) (c:coalition) (ss:strategy_set g q c) (l: list State) (CPL: computation_property g q l) : Prop *)
-(* := *)
-(*   forall (i:nat), *)
-(*     S i  < (length l) -> *)
-(*     forall (m:move_vec) *)
-(*            (p:Player) *)
-(*            (H: c p = true), *)
-(*     let x := firstn i l in *)
-(*     m (nth i l q) p = ss p H x CPL -> *)
-(*     g.(d) (nth i l q) m = (nth (S i) l q). *)
-
-
