ATL_prime.v
@@ -1,0 +1,164 @@
+(* Alternating-Time Temporal Logic - a version without negative Observables *)
+Require Export CGS.
+
+(* Inductive type of a sentence in (incomplete) propositional logic. *)
+Inductive prop_sentence : Set :=
+| obs : Observable -> prop_sentence
+| pand : prop_sentence -> prop_sentence -> prop_sentence
+| por :  prop_sentence -> prop_sentence -> prop_sentence.
+
+
+(* Inductive type of a sentence in ATL. *)
+Inductive sentence : Set :=
+| prop : prop_sentence -> sentence
+| possible_next : coalition -> sentence -> sentence
+| possible_once : coalition -> sentence -> sentence
+| possible_always : coalition -> sentence -> sentence
+| possible_until : coalition -> sentence -> sentence -> sentence
+| necessary_next : coalition -> sentence -> sentence
+| necessary_once : coalition -> sentence -> sentence
+| necessary_always : coalition -> sentence -> sentence
+| necessary_until : coalition -> sentence -> sentence -> sentence.
+
+(* Notation for ATl sentences. *)
+Notation "p //\\ q" := (pand p q) (at level 30).
+Notation "p \\// q" := (por p q) (at level 30).
+Notation "<< c >>o p" := (possible_next c p) (at level 50).
+Notation "<< c >>^ p" := (possible_once c  p) (at level 50).
+Notation "<< c >># p" := (possible_always c p) (at level 50).
+Notation "<< c >> p %% q" := (possible_until c p q) (at level 50).
+Notation "[[ c ]]o p" := (necessary_next c p) (at level 50).
+Notation "[[ c ]]^ p" := (necessary_once c p) (at level 50).
+Notation "[[ c ]]# p" := (necessary_always c p)  (at level 50).
+Notation "[[ c ]] p %% q" := (necessary_until c p q) (at level 50).
+
+Inductive prop_verifies : CGS -> State -> prop_sentence -> Prop :=
+| verifiesObs : forall (g:CGS) (q:State) (a:Observable),
+    beq_observable (g.(o) q) a = true ->
+    prop_verifies g q (obs a)
+| verifiesAnd : forall (g:CGS) (q:State) (phi psi : prop_sentence),
+    (prop_verifies g q phi /\ prop_verifies g q psi) ->
+    prop_verifies g q (phi //\\ psi)
+| verifiesOr : forall (g:CGS) (q:State) (phi psi : prop_sentence),
+    (prop_verifies g q phi \/ prop_verifies g q psi) ->
+    prop_verifies g q (phi \\// psi).
+
+Inductive verifies: CGS -> State -> sentence -> Prop :=
+| verifiesPossibleNext: forall (g: CGS) (q: State) (phi: sentence) (c:coalition),
+    (exists (ss:strategy_set g c),
+        forall (l:Stream State) (CPL: computation_property g q l),
+          outcomes g c ss l ->
+          verifies g (Str_nth 1 l) phi) ->
+    verifies g q (<<c>>o phi)
+| verifiesPossibleOnce: forall (g: CGS) (q: State) (phi: sentence) (c:coalition),
+    (exists (ss:strategy_set g c),
+        forall (l:Stream State) (CPL: computation_property g q l),
+          outcomes g c ss l ->
+          (exists n:nat, verifies g (Str_nth n l) phi)) ->
+    verifies g q (<<c>>^ phi)
+| verifiesPossibleAlways: forall (g: CGS) (q: State) (phi: sentence) (c:coalition),
+    (exists (ss:strategy_set g c),
+        forall (l:Stream State) (CPL: computation_property g q l),
+                  outcomes g c ss l ->
+          (forall n:nat, verifies g (Str_nth n l) phi)) ->
+    verifies g q (<<c>># phi)
+| verifiesPossibleUntil : forall (g: CGS) (q: State) (phi psi: sentence) (c:coalition),
+    (exists (ss:strategy_set g c),
+        forall (l:Stream State) (CPL: computation_property g q l),
+          outcomes g c ss l ->
+          (exists (n:nat),
+              (verifies g (Str_nth n l) psi) /\
+              (forall m:nat, verifies g (Str_nth m l) phi))) ->
+    verifies g q (<<c>> phi %% psi)
+| verifiesNecessaryNext: forall (g: CGS) (q: State) (phi: sentence) (c:coalition),
+    (forall (ss:strategy_set g c),
+        exists (l:Stream State) (CPL: computation_property g q l),
+          outcomes g c ss l /\
+          verifies g (Str_nth 1 l) phi) ->
+    verifies g q ([[c]]o phi)
+| verifiesNecessaryOnce: forall (g: CGS) (q: State) (phi: sentence) (c:coalition),
+    (forall (ss:strategy_set g c),
+        exists (l:Stream State) (CPL: computation_property g q l),
+          outcomes g c ss l /\
+          (exists n:nat, verifies g (Str_nth n l) phi)) ->
+    verifies g q ([[c]]^ phi)
+| verifiesNecessaryAlways: forall (g: CGS) (q: State) (phi: sentence) (c:coalition),
+    (forall (ss:strategy_set g c),
+        exists (l:Stream State) (CPL: computation_property g q l),
+          outcomes g c ss l /\
+          (forall n:nat, verifies g (Str_nth n l) phi)) ->
+    verifies g q ([[c]]# phi)
+| verifiesNecessaryUntil : forall (g: CGS) (q: State) (phi psi: sentence) (c:coalition),
+    (forall (ss:strategy_set g c),
+        exists (l:Stream State) (CPL: computation_property g q l),
+          outcomes g c ss l /\
+          (exists (n:nat),
+              (verifies g (Str_nth n l) psi) /\
+              (forall m:nat, verifies g (Str_nth m l) phi))) ->
+    verifies g q (<<c>> phi %% psi).
+
+
+    
+    
+Definition invariant (g1 g2:CGS) : Prop := forall (phi:sentence) (q:State),
+    verifies g1 q phi <-> verifies g2 q phi.
+    
+(* TODO: invariance. *)
+(* TODO: proof calculus *)
+
+Definition spec : Type := State -> sentence -> Prop.
+
+Definition g_in_spec (sp:spec) (g:CGS) (q:State) : Prop := forall (phi:sentence), sp q phi -> verifies g q phi.
+
+
+Theorem coal_comp_comp : forall c, coal_comp (coal_comp c) = c.
+Proof.
+  intros.
+  unfold coal_comp. intros. apply functional_extensionality. intros. destruct (c x).
+  - reflexivity.
+  - reflexivity.
+Qed.
+  
+Axiom d_sentence : forall (g:CGS) (q:State) (phi:sentence), decidable (verifies g q phi).
+
+
+
+Theorem coalition_complement_next : forall (g:CGS) (q:State) (phi:sentence) (c:coalition),
+    verifies g q (<<c>>o phi) <-> verifies g q ([[coal_comp c]]o phi).
+Proof.
+Admitted.
+  (* intros. split. *)
+  (* - intros. inversion H. apply verifiesNecessaryNext. *)
+  (*   pose proof (H3 (sq q) (computation_property_sq g q)). *)
+  (*   destruct H5. *)
+  (*   exists (sq q). exists (computation_property_sq g q). intros. *)
+  (*   assert (outcomes g c x (sq q)). *)
+  (*   { *)
+  (*     cofix OUT'. destruct (sq q), s0. *)
+  (*     inversion OUT'. *)
+  (*     apply (outcomes_cons g c x s s0 _ m CPL ENABLED DELTA OUT ). *)
+  (*   } *)
+  (*   apply H5 in H6. *)
+  (*   split. *)
+  (*   + cofix H7. destruct (sq q), s0. *)
+  (*     inversion H7. *)
+  (*     apply (outcomes_cons g (coal_comp c) ss s s0 _ m CPL ENABLED DELTA OUT). *)
+  (*   + apply H6. *)
+  (* - intros. inversion H. apply verifiesPossibleNext. *)
+  (*   intros. *)
+  (*   destruct H3, H3. *)
+    
+Theorem coalition_complement_once_always : forall (g:CGS) (q:State) (phi:sentence) (c:coalition),
+    verifies g q (<<c>>^ phi) <-> verifies g q ([[coal_comp c]]^ phi).
+Proof.
+Admitted.
+
+Theorem coalition_complement_until : forall (g:CGS) (q:State) (phi psi:sentence) (c:coalition),
+    verifies g q (<<c>> phi %% psi) <-> verifies g q ([[coal_comp c]] phi %% psi).
+Proof.
+Admitted.
+
+(* Create HintDb verifies. *)
+(* Hint Resolve coalitiion_complement_next : verifies. *)
+
+(* auto with verifies *)
